examples/store_sess/proofs/client/load.v
@@ -1,0 +1,95 @@
+From stdpp Require Import base gmap.
+From mathcomp Require Import ssreflect.
+From stdpp Require Import namespaces.
+From iris.algebra Require Import agree auth csum gset gmap excl frac.
+From iris.algebra Require Import max_prefix_list dfrac_agree.
+From iris.base_logic Require Import invariants.
+From iris.heap_lang Require Import notation proofmode.
+From iris.heap_lang.lib Require Import ticket_lock.
+From cryptis Require Import lib term gmeta nown cryptis.
+From cryptis Require Import replica primitives tactics role.
+From cryptis.examples Require Import iso_dh gen_conn sess.
+From cryptis.examples.sess Require impl.
+From cryptis.examples.sess.proofs Require Import base.
+From cryptis.examples.sess Require Import proofs tag.
+From cryptis.examples.store Require Import db.
+From cryptis.examples.store_sess Require Import impl.
+From cryptis.examples.store_sess.proofs Require Import base.
+From actris.channel Require Import proto_model proto.
+
+Set Implicit Arguments.
+Unset Strict Implicit.
+Unset Printing Implicit Defensive.
+
+Local Existing Instance ticket_lock.
+
+Section Verif.
+
+Context `{!cryptisGS Σ, !heapGS Σ, !iso_dhGS Σ, !GenConn.connGS Σ,
+          !sessG Σ, !storeGS Σ, !tlockG Σ}.
+Notation iProp := (iProp Σ).
+
+Implicit Types (cs : GenConn.state).
+Implicit Types (skI skR : sign_key) (kS t : term).
+Implicit Types n : nat.
+Implicit Types γ : gname.
+Implicit Types (db : gmap term term).
+
+Lemma wp_client_load skI skR cs t1 t2 :
+  cryptis_ctx -∗
+  store_ctx -∗
+  public t1 -∗
+  {{{ db_connected skI skR cs ∗
+      db_mapsto skI skR t1 t2 }}}
+    Client.load (repr cs) t1
+  {{{ t2', RET (repr t2');
+      db_connected skI skR cs ∗
+      db_mapsto skI skR t1 t2 ∗
+      public t2' ∗
+      (compromised cs ∨ ⌜t2' = t2⌝) }}}.
+Proof.
+iIntros "#? #ctx #p_t1 !> %Φ [client mapsto] post".
+iDestruct "client" as "(%db & conn & rel & ready & state)".
+iPoseProof (DB.db_state_mapsto with "state mapsto") as "%Hk".
+wp_lam; wp_pures.
+wp_bind (tag _ _). iApply wp_tag.
+wp_bind (Sess.send _ _).
+iApply (wp_send_msg _ _ _ _
+          (iMsg_tag (db_arms skI skR cs (db_st skI skR cs) db)) _
+          (<? v> MSG v {{ ⌜db !! t1 = Some v⌝ }};
+             db_st skI skR cs db)%proto
+          with "[conn]").
+{ iSplitL "conn".
+  { iApply (connected_le with "conn"). iNext.
+    iApply iProto_le_of_equiv. exact: db_st_unfold. }
+  iSplitR; first by rewrite public_tag.
+  iRight.
+  iApply (iMsg_tag_intro _ _ (db_arms_load _ _ _ _ _)).
+  rewrite iMsg_exist_eq /=. iExists t1.
+  rewrite iMsg_base_eq /=.
+  iSplit; first done.
+  iSplit; first by eauto.
+  auto. }
+iIntros "!> conn". wp_pures.
+iApply wp_fupd.
+wp_apply (wp_recv with "conn").
+iIntros "%t2' %p' (#p_t2' & conn & disj)".
+iDestruct (connected_public_key_or' with "conn rel disj")
+  as "(conn & rel & >disj)".
+iDestruct "disj" as "[#comp|car]".
+- iModIntro. iApply "post". iFrame "mapsto p_t2'".
+  iSplitL; last by iLeft.
+  iExists db. iFrame "rel ready state".
+  by iApply (connected_compromised with "conn comp").
+- rewrite iMsg_exist_eq /=. iDestruct "car" as "(%v & car)".
+  rewrite iMsg_base_eq /=.
+  iDestruct "car" as "(-> & Heq & %Hv)".
+  rewrite later_equivI_1.
+  iModIntro. iApply "post". iFrame "mapsto p_t2'".
+  iSplitL; last by rewrite Hk in Hv; case: Hv => ->; iRight.
+  iExists db. iFrame "rel ready state".
+  iApply (connected_le with "conn"). iNext.
+  iRewrite -"Heq". iApply iProto_le_refl.
+Qed.
+
+End Verif.
